clean up

Semantics/Imp/Lang.lean
@@ -3,16 +3,17 @@ import Semantics.Maps
 @[reducible]
 def Val := Int
 
-def State := total_map Val
-def State.nil: State := total_map.default 0
+def State := TotalMap Val
+def State.nil: State := TotalMap.default 0
 
 notation "σ₀" => State.nil
 
-#reduce σ₀ "x"
-#reduce (σ₀⟪"x" ≔ 3⟫⟪"x" ≔ 4⟫) "x"
-#reduce (σ₀⟪"x" ≔ 3⟫⟪"x" ≔ 4⟫⟪"x" ≔ 7⟫) "x"
+#eval σ₀ "x"
+#eval (σ₀⟪"x" ≔ 3⟫⟪"x" ≔ 4⟫) "x"
+#eval (σ₀⟪"x" ≔ 3⟫⟪"x" ≔ 4⟫⟪"x" ≔ 7⟫) "x"
 
-theorem State.demo₁: σ₀⟪"x" ≔ 3⟫ = σ₀⟪"x" ≔ 4⟫⟪"x" ≔ 3⟫ := by sorry
+theorem State.demo₁: σ₀⟪"x" ≔ 3⟫ = σ₀⟪"x" ≔ 4⟫⟪"x" ≔ 3⟫ := by
+  simp
 
 inductive Aexp where
   | val : Val → Aexp
