Semantics/Maps.lean
@@ -6,27 +6,133 @@
 ## Total maps
 -/
 
-def total_map A := String → A
+def TotalMap A := String → A
 
-def total_map.default (v: A): total_map A := λ _ ↦ v
+def TotalMap.default (v: A): TotalMap A := λ _ ↦ v
 
-def total_map.update (m: total_map A) (x: String) (v: A) :=
-  λ y ↦ bif x = y then v else m y
+def TotalMap.update (map: TotalMap A) (key: String) (val: A) :=
+  λ key' ↦ if key = key' then val else map key'
 
-notation m "⟪" x " ≔ " v "⟫" => total_map.update m x v
+notation map "⟪" key " ≔ " val "⟫" => TotalMap.update map key val
+
+@[simp] theorem update_apply (key : String) (val : A) (map : TotalMap A) :
+  (map⟪key ≔ val⟫) key = val :=
+  by
+    apply if_pos
+    rfl
+
+@[simp] theorem update_apply_neq (key key' : String) (val : A) (map : TotalMap A)
+    (hneq : key ≠ key'):
+    (map⟪key ≔ val⟫) key' = map key' :=
+    by
+      apply if_neg
+      assumption
+
+@[simp] theorem update_override (name : String) (val₁ val₂ : A) (s : TotalMap A) :
+  s⟪name ≔ val₂⟫⟪name ≔ val₁⟫ = s⟪name ≔ val₁⟫ :=
+  by
+    apply funext
+    intro name'
+    cases Classical.em (name' = name) with
+    | inl h =>
+      cases h
+      rw [update_apply, update_apply]
+    | inr h =>
+      rw [update_apply_neq]
+      . rw [update_apply_neq]
+        . rw [update_apply_neq]
+          rw [ne_comm, ne_eq]
+          exact h
+        . rw [ne_comm, ne_eq]
+          exact h
+      . rw [ne_comm, ne_eq]
+        exact h
+
+@[simp] theorem update_swap (name₁ name₂ : String) (val₁ val₂ : A) (s : TotalMap A)
+    (hneq : name₁ ≠ name₂) :
+  s⟪name₂ ≔ val₂⟫⟪name₁ ≔ val₁⟫ = s⟪name₁ ≔ val₁⟫⟪name₂ ≔ val₂⟫ :=
+  by
+    apply funext
+    intro name'
+    cases Classical.em (name' = name₁) with
+    | inl h =>
+      cases h
+      rw [update_apply, update_apply_neq]
+      . rw [update_apply]
+      . rw [ne_comm]
+        exact hneq
+    | inr h =>
+      cases Classical.em (name' = name₁) with
+      | inl h₁ =>
+        cases h₁
+        rw [eq_self] at h
+        contradiction
+      | inr h₁ =>
+        cases Classical.em (name' = name₂) with
+        | inl h₂ =>
+          cases h₂
+          rw [update_apply, update_apply_neq]
+          . rw [update_apply]
+          . rw [ne_comm, ne_eq]
+            exact h
+        | inr h₂ =>
+          rw [update_apply_neq]
+          . rw [update_apply_neq]
+            . rw [update_apply_neq]
+              . rw [update_apply_neq]
+                rw [ne_comm, ne_eq]
+                exact h
+              . rw [ne_comm, ne_eq]
+                exact h₂
+            . rw [ne_comm, ne_eq]
+              assumption
+          . rw [ne_comm, ne_eq]
+            exact h
+
+@[simp] theorem update_id (name : String) (s : TotalMap A) :
+  s⟪name ≔ s name⟫ = s :=
+  by
+    apply funext
+    intro name'
+    cases Classical.em (name' = name) with
+    | inl h =>
+      cases h
+      rw [update_apply]
+    | inr h =>
+      rw [update_apply_neq]
+      rw [ne_comm, ne_eq]
+      exact h
+
+@[simp] theorem update_same_const (name : String) (val : A) :
+  (λ _ ↦ val)⟪name ≔ val⟫ = (λ _ ↦ val) :=
+  by
+    apply funext
+    intro name'
+    cases Classical.em (name' = name) with
+    | inl h =>
+      cases h
+      rw [update_apply]
+    | inr h =>
+      rw [update_apply_neq]
+      rw [ne_comm, ne_eq]
+      exact h
+
+example (map : TotalMap Nat) :
+  map⟪"a" ≔ 0⟫⟪"a" ≔ 2⟫ = map⟪"a" ≔ 2⟫ :=
+  by simp
+
+example (map : TotalMap Nat) :
+  map⟪"a" ≔ 0⟫⟪"b" ≔ 2⟫ = map⟪"b" ≔ 2⟫⟪"a" ≔ 0⟫ :=
+  by simp
+
+example (map : TotalMap Nat) :
+  map⟪"a" ≔ map "a"⟫⟪"b" ≔ 0⟫ = map⟪"b" ≔ 0⟫ :=
+  by simp
 
 /-
 ## Partial maps
 -/
 
-def partial_map A := total_map $ Option A
+def PartialMap A := TotalMap (Option A)
 
-def partial_map.default: partial_map A := λ _ ↦ none
-
-def includedin (a b: partial_map A) := ∀ x v, (a x = some v) → (b x = some v)
-
-theorem includedin_update x v (h: includedin a b):
-  includedin (a ⟪x ≔ some v⟫) (b ⟪x ≔ some v⟫) :=  by
-  {
-    sorry
-  }
+def PartialMap.default: PartialMap A := TotalMap.default none
