lakefile.lean
@@ -1,14 +1,15 @@
 import Lake
 open Lake DSL
 
-package «imp» {
-  -- add any package configuration options here
-}
+package "semantics" where
+  -- Settings applied to both builds and interactive editing
+  leanOptions := #[
+    ⟨`pp.unicode.fun, true⟩ -- pretty-prints `fun a ↦ b`
+  ]
+  -- add any additional package configuration options here
 
-require mathlib from git
-  "https://github.com/leanprover-community/mathlib4.git"
+require "leanprover-community" / "mathlib"
 
 @[default_target]
-lean_lib «Semantics» {
+lean_lib «Semantics» where
   -- add any library configuration options here
-}
